test/coq/arith_proof.v
@@ -67,28 +67,7 @@ Axiom int_representable:
    improve the proof --- especially the way to handle mutually recursive
    functions. *)
 
-(* -------------------------------------------------------------------------- *)
-
-(* Sixth version: It should no longer be necessary to provide en environment [η]
-                  which contains the standard library as a module. *)
-
-(* -------------------------------------------------------------------------- *)
-
-(* Fifth version: Once the specifications proven, the [wp] tactic should know
-                  how to handle them (ie. use their spec as soon as possible,
-                  and handle their partial applications automatically!). *)
-
-(* -------------------------------------------------------------------------- *)
-
-(* Fourth version: The process of declaring specifications should be
-                   interactive. *)
-
-(* -------------------------------------------------------------------------- *)
-
-(* Third version: a lemma exists to better reason on mutually recursive
-                  functions. *)
-
-Lemma Add_spec3 :
+Lemma Add_spec :
     let Λ :=
     [
       ("add", add_spec);
@@ -100,82 +79,13 @@ Lemma Add_spec3 :
            EnvNil in
   ⊢ WP eval_mexpr η Arith {{ module_spec Λ }}.
 Proof.
-  intros.
-  wp.
+  intros. wp.
 
-  oSpecify "add" add_spec vadd "#Hadd"
-           "mult" mult_spec mult "#Hmult".
+  o_specify "add" add_spec "#Hadd"
+            "mult" mult_spec "#Hmult".
 
   (* Specification of the addition. *)
-  { (* The rest of the proof is unchanged. *) admit. }
-
-  (* Specification of the multiplication. *)
-  { (* The rest of the proof is unchanged. *) admit. }
-
-  (* The rest of the proof is unchanged. *)
-Admitted.
-
-(* -------------------------------------------------------------------------- *)
-
-(* Second version: the values of [add] and [mult] are opacified manually at "the
-                   right time". *)
-
-Lemma Add_spec2 :
-    let Λ :=
-    [
-      ("add", add_spec);
-      ("mult", mult_spec);
-      ("i3", is_equal #3)
-    ]
-  in
-  let η := EnvCons "Stdlib" Stdlib $
-           EnvNil in
-  ⊢ WP eval_mexpr η Arith {{ module_spec Λ }}.
-Proof.
-  intros.
-  wp.
-
-  (* [add] and [mult] are recursively defined.
-     Intuitively, one wants:
-     1. to provide the required specs for the environment;
-     2. to prove each spec one by one using Löb Induction.
-
-     Although it is not the case here, it might also be necessary to provide
-     external hypotheses to prove the specs.
-
-     The following does *not* work as expected. As the [RecBinding]s take
-     functions as argument and we only generalize values in the current process,
-     the specs hidden behind the [▷] are unusable (and useless).
-     Therefore, one should abstract the bodies of the function, and prove a spec
-     for them. *)
-
-  lazymatch goal with
-  | |- environments.envs_entails
-         ?Δ (wp ?s ?E
-                (ret_dconcat
-                   (EnvCons "add" ?vadd $
-                            EnvCons "mult" ?vmult $
-                            EnvNil)
-                   ?δη)
-                ?φ) =>
-      iAssert (add_spec vadd ∗ mult_spec vmult ∗ emp)%I as "(#Hadd & #Hmult & _)"
-  end;
-  [ (* In order to prove the assertion, we use Löb induction. *)
-    iLöb as "IH";
-    iDestruct "IH" as "(#Hadd&#Hmult&_)";
-    iSplitL "" ; (* Proving the addition does not require prior resources. *)
-    [
-    | iSplitL "";
-      [
-      | done ]
-    ]
-  | (* After the specifications have been proven, abstract the addition and
-       multiplication and .continue. *)
-    oAbstract "add" vadd; oAbstract "mult" vmult; wp_continue ].
-
-  { (* ---------------------------------------------------------------------- *)
-    (* Proof of [add]. *)
-    { iModIntro. iIntros(i1 H1).
+  { iModIntro. iIntros(i1 H1).
 
       (* It is during the function call to add that the environment is extended
          to include the definition of [mult].*)
@@ -213,252 +123,58 @@ Proof.
           iSpecialize ("Hadd1" $! (i1 + (i2 - 1))%Z NotStuck top). wp.
           iApply (wp_covariant with "Hadd1").
           iIntros (?->).
-          iPureIntro. do 2 f_equal. lia. } } } }
-
-    (* ------------------------------------------------------------------ *)
-    (* Proof of [mult]. *)
-    { iModIntro. iIntros (i1 H1).
-
-      (* It is during the function call to add that the environment is extended
-         to include the definition of [mult].*)
-      oCall "add" vadd "mult" vmult. wp_continue.
-
-      (* The proof can now continue as expected. *)
-      iIntros(i2 H2). wp. wp_continue.
-      wp_use Stdlib__eq__spec; try done; try apply int_representable.
-      iIntros (veq_part) "Heq_part".
-      wp. iApply (wp_covariant with "Heq_part").
-      iIntros (?->).
-      destruct (i2 =? 0)%Z eqn:E.
-      { (* [i2 = 0%Z]. *) wp.
-        apply Z.eqb_eq in E as ->. iPureIntro. do 2 f_equal. lia. }
-      { (* [i2 != 0%Z]. *) wp.
-        wp_use Stdlib__eq__spec; try done; try apply int_representable.
-        clear veq_part.
-        iIntros (veq_part) "Heq_part".
-        wp. iApply (wp_covariant with "Heq_part").
-        iIntros (?->).
-        destruct (i2 =? 1)%Z eqn:E1.
-        { (* [i2 = 1%Z]. *) wp.
-          apply Z.eqb_eq in E1 as ->. iPureIntro. do 2 f_equal. lia. }
-        { (* [i2 <> 1%Z]. *) wp.
-          (* Proof that [add x (mult x (y - 1)) == x * y]. *)
-          wp_par.
-          { (* [λ y, add x y]. *)
-            iSpecialize ("Hadd" $! i1 H1).
-            wp_use "Hadd". }
-          { (* [mult x (y - 1)] *)
-            wp_par.
-            { (* [λ y, mult x y]. *)
-              wp_use "Hmult"; iPureIntro; exact H1. }
-            { (* [y - 1]. *) wp_call.
-              by instantiate (1 := λ v, ⌜ v = # (i2 - 1)%Z ⌝%I). }
-            { iIntros (vmult_part ?) "Hmult_part ->".
-              wp. wp_use "Hmult_part".
-              iPureIntro. lia. } }
-          { (* Finish the application of [add]. *)
-            iIntros (vadd_part ?) "Hadd_part ->".
-            wp.
-            unshelve iSpecialize ("Hadd_part" $! (i1 * (i2 - 1))%Z _).
-            { apply Ztac.mul_le; lia. }
-            iApply (wp_covariant with "Hadd_part").
-            iIntros (?->).
-            iPureIntro. do 2 f_equal.
-            lia. } } } }
-
-  wp_par;
-    [ wp_use "Hadd"; done
-    | wp_use "Hadd";
-      [ done | iIntros (vadd_part) "Hadd_part"; wp; by iApply "Hadd_part" ]
-    | ].
-  iIntros (vadd_part ?) "Hadd_part ->". wp.
-  iSpecialize("Hadd_part" $! _ _).
-  iApply (wp_covariant with "Hadd_part").
-  Unshelve. 2: lia.
-  iIntros (?->). wp.
-  wp_specify "i3" (is_equal #3); first done.
-  iIntros (i3) "#Hi3". wp_continue.
-
-  repeat wp_par.
-  { wp_use "Hmult"; first done.
-    iIntros (vmult_part) "Hmult_part".
-    iSpecialize ("Hmult_part" $! _ _). wp.
-    iApply (wp_covariant with "Hmult_part").
-    iIntros (?->).
-    wp_use "Hadd"; first done. }
-  { wp_use "Hadd"; first done. }
-  { wp_use "Hmult"; first done. }
-  { wp_use "Hadd"; first done.
-    iIntros (vadd_part') "Hadd_part'".
-    iSpecialize ("Hadd_part'" $! _ _).
-    iApply (wp_covariant with "Hadd_part'").
-    iIntros(?->). by wp_set_postcondition. }
-  { iIntros (v1 ?) "H1 ->". wp.
-    iSpecialize ("H1" $! _ _).
-    iApply (wp_covariant with "H1").
-    iIntros (?->). by wp_set_postcondition. }
-  { iIntros (v1 ?) "H1 ->". wp.
-    iSpecialize ("H1" $! _ _).
-    iApply (wp_covariant with "H1").
-    iIntros (?->). by wp_set_postcondition. }
-  { iIntros (v1 ?) "H1 ->". wp.
-    iSpecialize ("H1" $! _ _).
-    iApply (wp_covariant with "H1").
-    iIntros (?->). wp. wp_continue.
-
-    wp_module_spec. }
-
-  Unshelve.
-  all: done.
-Time Qed.
-
-(* -------------------------------------------------------------------------- *)
-
-(* Initial version: the values of [add] and [mult] are abstracted away after
-                    having proven their specifications. Unfortunately, [add]
-                    (resp. [mult]) is not opaque when proving [mult]
-                    (resp. [add]). *)
-Lemma Add_spec :
-    let Λ :=
-    [
-      ("add", add_spec);
-      ("mult", mult_spec);
-      ("i3", is_equal #3)
-    ]
-  in
-  let η := EnvCons "Stdlib" Stdlib $
-           EnvNil in
-  ⊢ WP eval_mexpr η Arith {{ module_spec Λ }}.
-Proof.
-  intros.
-  wp.
-
-  (* [add] and [mult] are recursively defined.
-     Intuitively, one wants:
-     1. to provide the required specs for the environment;
-     2. to prove each spec one by one using Löb Induction.
-
-     Although it is not the case here, it might also be necessary to provide
-     external hypotheses to prove the specs.
-
-     The following does *not* work as expected. As the [RecBinding]s take
-     functions as argument and we only generalize values in the current process,
-     the specs hidden behind the [▷] are unusable (and useless).
-     Therefore, one should abstract the bodies of the function, and prove a spec
-     for them. *)
-
-  lazymatch goal with
-  | |- environments.envs_entails
-         ?Δ (wp ?s ?E
-                (ret_dconcat
-                   (EnvCons "add" ?vadd $
-                            EnvCons "mult" ?vmult $
-                            EnvNil)
-                   ?δη)
-                ?φ) =>
-      iAssert (add_spec vadd ∗ mult_spec vmult ∗ emp)%I as "H"
-  end.
-  (* [_ ∗ emp] allows to better understand how the process would work with more
-     functions. *)
-  { iLöb as "IH".
-    iSplitL "".
-    (* ---------------------------------------------------------------------- *)
-    (* Proof of [add]. *)
-    { iRevert "IH" (* ;
-        lazymatch goal with
-        | |- context [VCloRec η ?rbds "mult"] =>
-            generalize (VCloRec η rbds "mult")
-        end *) .
-      iIntros (* vmult *) "(#Hadd&#Hmult&_) !>".
-      iIntros(i1 H1). wp_call. wp_continue. iIntros(i2 H2). wp. wp_continue.
-      wp_use Stdlib__eq__spec; try done; try apply int_representable.
-      iIntros (veq_part) "Hspec_eq".
-      wp.
-      iApply (wp_covariant with "Hspec_eq"). (* TODO: fix [wp_use]. *)
-      iIntros (? ->).
-      destruct (i2 =? 0)%Z eqn:E; wp.
-      { (* [i2 = 0%Z] *)
-        apply Z.eqb_eq in E as ->.
-        wp_use "Hmult"; first done.
-        iIntros (Hmult_part) "Hmult_part".
-        iApply (wp_covariant with "[Hmult_part]").
-        { iApply "Hmult_part"; done. }
-        iIntros(?->).
-        iPureIntro. do 2 f_equal. lia. }
-      { (* [i2 != 0%Z], goal: [1 + (add x (y - 1)) == x + y] *)
-        wp_par.
-        { (* [λ y, 1 + y] *) iIntros (vpartial) "H". iExact "H". }
-        { (* [add x (y - 1)]. *)
-          wp_par.
-          { wp_use "Hadd"; iPureIntro; exact H1. }
-          - wp_call.
-            by instantiate (1 := λ v, ⌜ v = # (i2 - 1)%Z ⌝%I).
-          - iIntros (vpadd ?) "Hadd_partial ->".
-            wp_use "Hadd_partial".
-            iPureIntro. lia. }
-        { iIntros (vadd1 ?) "Hadd1 ->".
-          wp.
-          iSpecialize ("Hadd1" $! (i1 + (i2 - 1))%Z NotStuck top). wp.
-          iApply (wp_covariant with "Hadd1").
-          iIntros (?->).
           iPureIntro. do 2 f_equal. lia. } } }
 
-    iSplitL "".
-    (* ------------------------------------------------------------------ *)
-    (* Proof of [mult]. *)
-    { iRevert "IH"(* ;
-        lazymatch goal with
-        | |- context [VCloRec η ?rbds "add"] =>
-             generalize (VCloRec η rbds "add")
-        end *) .
-      iIntros (* vadd *) "(#Hadd&#Hmult&_) !>".
-      iIntros (i1 H1). wp_call. wp_continue.
-      iIntros(i2 H2). wp. wp_continue.
+  (* ------------------------------------------------------------------ *)
+  (* Specification of the multiplication. *)
+  { iModIntro. iIntros (i1 H1).
+
+    (* It is during the function call to add that the environment is extended
+         to include the definition of [mult].*)
+    oCall "add" vadd "mult" vmult. wp_continue.
+
+    (* The proof can now continue as expected. *)
+    iIntros(i2 H2). wp. wp_continue.
+    wp_use Stdlib__eq__spec; try done; try apply int_representable.
+    iIntros (veq_part) "Heq_part".
+    wp. iApply (wp_covariant with "Heq_part").
+    iIntros (?->).
+    destruct (i2 =? 0)%Z eqn:E.
+    { (* [i2 = 0%Z]. *) wp.
+      apply Z.eqb_eq in E as ->. iPureIntro. do 2 f_equal. lia. }
+    { (* [i2 != 0%Z]. *) wp.
       wp_use Stdlib__eq__spec; try done; try apply int_representable.
+      clear veq_part.
       iIntros (veq_part) "Heq_part".
       wp. iApply (wp_covariant with "Heq_part").
       iIntros (?->).
-      destruct (i2 =? 0)%Z eqn:E.
-      { (* [i2 = 0%Z]. *) wp.
-        apply Z.eqb_eq in E as ->. iPureIntro. do 2 f_equal. lia. }
-      { (* [i2 != 0%Z]. *) wp.
-        wp_use Stdlib__eq__spec; try done; try apply int_representable.
-        clear veq_part.
-        iIntros (veq_part) "Heq_part".
-        wp. iApply (wp_covariant with "Heq_part").
-        iIntros (?->).
-        destruct (i2 =? 1)%Z eqn:E1.
-        { (* [i2 = 1%Z]. *) wp.
-          apply Z.eqb_eq in E1 as ->. iPureIntro. do 2 f_equal. lia. }
-        { (* [i2 <> 1%Z]. *) wp.
-          (* Proof that [add x (mult x (y - 1)) == x * y]. *)
+      destruct (i2 =? 1)%Z eqn:E1.
+      { (* [i2 = 1%Z]. *) wp.
+        apply Z.eqb_eq in E1 as ->. iPureIntro. do 2 f_equal. lia. }
+      { (* [i2 <> 1%Z]. *) wp.
+        (* Proof that [add x (mult x (y - 1)) == x * y]. *)
+        wp_par.
+        { (* [λ y, add x y]. *)
+          iSpecialize ("Hadd" $! i1 H1).
+          wp_use "Hadd". }
+        { (* [mult x (y - 1)] *)
           wp_par.
-          { (* [λ y, add x y]. *)
-            iSpecialize ("Hadd" $! i1 H1).
-            wp_use "Hadd". }
-          { (* [mult x (y - 1)] *)
-            wp_par.
-            { (* [λ y, mult x y]. *)
-              wp_use "Hmult"; iPureIntro; exact H1. }
-            { (* [y - 1]. *) wp_call.
-              by instantiate (1 := λ v, ⌜ v = # (i2 - 1)%Z ⌝%I). }
-            { iIntros (vmult_part ?) "Hmult_part ->".
-              wp. wp_use "Hmult_part".
-              iPureIntro. lia. } }
-          { (* Finish the application of [add]. *)
-            iIntros (vadd_part ?) "Hadd_part ->".
-            wp.
-            unshelve iSpecialize ("Hadd_part" $! (i1 * (i2 - 1))%Z _).
-            { apply Ztac.mul_le; lia. }
-            iApply (wp_covariant with "Hadd_part").
-            iIntros (?->).
-            iPureIntro. do 2 f_equal.
-            lia. } } } }
-    done. }
-  oAbstract "add" vadd
-            "mult" vmult.
-  iDestruct "H" as "(#Hadd & #Hmult & _)".
-  wp_continue.
+          { (* [λ y, mult x y]. *)
+            wp_use "Hmult"; iPureIntro; exact H1. }
+          { (* [y - 1]. *) wp_call.
+            by instantiate (1 := λ v, ⌜ v = # (i2 - 1)%Z ⌝%I). }
+          { iIntros (vmult_part ?) "Hmult_part ->".
+            wp. wp_use "Hmult_part".
+            iPureIntro. lia. } }
+        { (* Finish the application of [add]. *)
+          iIntros (vadd_part ?) "Hadd_part ->".
+          wp.
+          unshelve iSpecialize ("Hadd_part" $! (i1 * (i2 - 1))%Z _).
+          { apply Ztac.mul_le; lia. }
+          iApply (wp_covariant with "Hadd_part").
+          iIntros (?->).
+          iPureIntro. do 2 f_equal.
+          lia. } } } }
 
   wp_par;
     [ wp_use "Hadd"; done
@@ -470,8 +186,7 @@ Proof.
   iApply (wp_covariant with "Hadd_part").
   Unshelve. 2: lia.
   iIntros (?->). wp.
-  wp_specify "i3" (is_equal #3); first done.
-  iIntros (i3) "#Hi3". wp_continue.
+  wp_continue.
 
   repeat wp_par.
   { wp_use "Hmult"; first done.
@@ -505,3 +220,5 @@ Proof.
   Unshelve.
   all: done.
 Time Qed.
+(* This [Qed.] is about 2.8s, while it was 2.0s with a manual iAssert.
+   TODO: improve the lemma applied by [oSpecify] to get better results! *)
